games/RTS.v
@@ -2,6 +2,7 @@ Require Import LogicalRelations.
 Require Import Axioms.
 Require Import Classical.
 Require Import Sets.
+Require Import KLR.
 
 (** * Prerequisites *)
 
@@ -21,6 +22,41 @@ Inductive move {G} :=
   | output_move (m : output G) :> move.
 
 Arguments move : clear implicits.
+
+(** Abstraction relation between two games *)
+
+Record abrel (G1 G2 : game) :=
+  {
+    abr_state : Type;
+    abr_init : abr_state;
+    abr_input : abr_state -> abr_state -> rel (input G1) (input G2);
+    abr_output : abr_state -> abr_state -> rel (output G1) (output G2);
+  }.
+
+Arguments abr_state {_ _}.
+Arguments abr_init {_ _}.
+Arguments abr_input {_ _}.
+Arguments abr_output {_ _}.
+
+Definition abr_id {G} : abrel G G :=
+  {|
+    abr_state := unit;
+    abr_init := tt;
+    abr_input w w' := eq;
+    abr_output w w' := eq;
+  |}.
+
+Definition abr_compose {GA GB GC} (GRAB : abrel GA GB) (GRBC : abrel GB GC) :=
+  {|
+    abr_state := abr_state GRAB * abr_state GRBC;
+    abr_init := (abr_init GRAB, abr_init GRBC);
+    abr_input :=
+      fun '(wab, wbc) '(wab', wbc') =>
+        rel_compose (abr_input GRAB wab wab') (abr_input GRBC wbc wbc');
+    abr_output :=
+      fun '(wab, wbc) '(wab', wbc') =>
+        rel_compose (abr_output GRAB wab wab') (abr_output GRBC wbc wbc');
+  |}.
 
 
 (** * Receptive transition systems *)
@@ -104,26 +140,32 @@ Module RTS.
   Definition cont G A :=
     input G -> set (resumption A).
 
-  Definition cont_le {G A B} R : rel (cont G A) (cont G B) :=
-    - ==> set_le (resumption_rel R).
+  Definition cont_le {GA GB A B} GR R w : rel (cont GA A) (cont GB B) :=
+    rforall w', abr_input GR w w' ++> set_le (resumption_rel (R w')).
 
-  Hint Extern 1 (RIntro _ (cont_le _) _ _) =>
-    eapply arrow_pointwise_rintro : typeclass_instances.
+  Hint Extern 1 (RIntro _ (cont_le _ _ _) _ _) =>
+    eapply rel_all_rintro : typeclass_instances.
 
-  Hint Extern 1 (RElim (cont_le _) _ _ _ _) =>
-    eapply arrow_pointwise_relim : typeclass_instances.
+  Hint Extern 1 (RElim (cont_le _ _ _) _ _ _ _) =>
+    eapply rel_all_relim; eexists : typeclass_instances.
 
-  Global Instance cont_le_refl {G} `(Reflexive) :
-    Reflexive (cont_le (G:=G) R).
+  Global Instance cont_le_refl {G A} R `{!forall w, @Reflexive A (R w)} w :
+    Reflexive (cont_le (@abr_id G) R w).
   Proof.
-    intros x q. reflexivity.
+    intros x w' q _ [ ]. reflexivity.
   Qed.
 
-  Global Instance cont_le_compose {G} `{RCompose} :
-    RCompose (cont_le RAB) (cont_le RBC) (cont_le (G:=G) RAC).
+  Global Instance cont_le_compose {GA GB GC A B C} GRAB GRBC RAB RBC RAC wab wbc :
+    (forall wab' wbc', @RCompose A B C (RAB wab') (RBC wbc') (RAC (wab', wbc'))) ->
+    RCompose
+      (cont_le GRAB RAB wab)
+      (cont_le GRBC RBC wbc)
+      (cont_le (@abr_compose GA GB GC GRAB GRBC) RAC (wab, wbc)).
   Proof.
-    intros k1 k2 k3 H12 H23 q.
-    rcompose (k2 q); eauto.
+    intros H k1 k2 k3 H12 H23 [w12' w23'] q1 q3 (q2 & Hq12 & Hq23).
+    specialize (H12 w12' q1 q2 Hq12).
+    specialize (H23 w23' q2 q3 Hq23).
+    rcompose (k2 q2); eauto.
   Qed.
 
   Definition cont_map {G A B} (f : A -> B) (k : cont G A) : cont G B :=
@@ -132,7 +174,9 @@ Module RTS.
   Global Instance cont_map_le :
     Monotonic
       (@cont_map)
-      (forallr -, forallr R, forallr S, (R ++> S) ++> cont_le R ++> cont_le S).
+      (forallr GR, forallr R : klr _, forallr S : klr _,
+        (rforall w, R w ++> S w) ++>
+        (rforall w, cont_le GR R w ++> cont_le GR S w)).
   Proof.
     unfold cont_map. rauto.
   Qed.
@@ -147,15 +191,16 @@ Module RTS.
 
   Arguments behavior : clear implicits.
 
-  Inductive behavior_le {G A B} R : rel (behavior G A) (behavior G B) :=
+  Inductive behavior_le {GA GB} GR {A B} R w : rel (behavior GA A) (behavior GB B) :=
     | internal_le :
-        Monotonic internal (R ++> behavior_le R)
-    | interacts_le :
-        Monotonic interacts (- ==> cont_le R ++> behavior_le R)
+        Monotonic internal (R w ++> behavior_le GR R w)
+    | interacts_le w' :
+        Monotonic interacts
+          (abr_output GR w w' ++> cont_le GR R w' ++> behavior_le GR R w)
     | diverges_le :
-        Monotonic diverges (behavior_le R)
+        Monotonic diverges (behavior_le GR R w)
     | goes_wrong_le ra :
-        Related ra goes_wrong (behavior_le R).
+        Related ra goes_wrong (behavior_le GR R w).
 
   Global Existing Instance internal_le.
   Global Existing Instance interacts_le.
@@ -164,21 +209,27 @@ Module RTS.
   Global Instance internal_le_params : Params (@internal) 1.
   Global Instance interacts_le_params : Params (@interacts) 2.
 
-  Global Instance behavior_le_refl {G A} (R: relation A) :
-    Reflexive R ->
-    Reflexive (behavior_le (G:=G) R).
+  Global Instance behavior_le_refl {G A} R w :
+    (forall w, @Reflexive A (R w)) ->
+    Reflexive (behavior_le (@abr_id G) R w).
   Proof.
-    intros H [a' | m k | | ]; constructor; eauto. intro. reflexivity.
+    intros H [a' | m k | | ]; try constructor; eauto.
+    - reflexivity.
+    - apply interacts_le with tt; simpl; repeat rstep.
+      destruct H0. reflexivity.
   Qed.
 
-  Global Instance behavior_le_compose {G} `{RCompose} :
-    RCompose (A := behavior G A)
-      (behavior_le RAB)
-      (behavior_le RBC)
-      (behavior_le RAC).
+  Global Instance behavior_le_compose {GA GB GC GRAB GRBC A B C RAB RBC RAC} wab wbc :
+    (forall wab wac, @RCompose A B C (RAB wab) (RBC wac) (RAC (wab, wac))) ->
+    RCompose
+      (behavior_le GRAB RAB wab)
+      (behavior_le GRBC RBC wbc)
+      (behavior_le (@abr_compose GA GB GC GRAB GRBC) RAC (wab, wbc)).
   Proof.
-    destruct 1; inversion 1; constructor; eauto.
-    ercompose; eauto.
+    intros H.
+    destruct 1; inversion 1; subst; try constructor; eauto.
+    - ercompose; eauto.
+    - apply interacts_le with (w', w'0); ercompose; rauto.
   Qed.
 
   Definition behavior_map {G A B} (f : A -> B) (r : behavior G A) :=
@@ -192,8 +243,9 @@ Module RTS.
   Global Instance behavior_map_le :
     Monotonic
       (@behavior_map)
-      (forallr -, forallr RA, forallr RB,
-        (RA ++> RB) ++> behavior_le RA ++> behavior_le RB).
+      (forallr GR, forallr RA : klr _, forallr RB : klr _,
+        (rforall w, RA w ++> RB w) ++>
+        (rforall w, behavior_le GR RA w ++> behavior_le GR RB w)).
   Proof.
     unfold behavior_map. rauto.
   Qed.
@@ -213,31 +265,35 @@ Module RTS.
     in the first has a correponding behavior in the second. In
     particular, internal transitions must correspond one-to-one. *)
 
-  Definition sim {G A B} (R : rel A B) : rel (rts G A) (rts G B) :=
-    (R ++> set_le (behavior_le R)).
+  Definition sim {GA GB} (GR : abrel GA GB) {A B} (R : klr _ A B) : rel (rts GA A) (rts GB B) :=
+    (rforall w, R w ++> set_le (behavior_le GR R w)).
 
-  Arguments sim {G A B} R%rel α%rts β%rts.
+  Arguments sim {GA GB} GR {A B} R%rel α%rts β%rts.
 
-  Hint Extern 1 (RElim (sim _) _ _ _ _) =>
-    eapply arrow_relim : typeclass_instances.
+  Hint Extern 1 (RElim (sim _ _ _) _ _ _ _) =>
+    eapply rel_all_relim : typeclass_instances.
 
   Hint Extern 1 (Transport _ _ _ (?α _ _) _) =>
     match type of α with rts _ _ => set_le_transport α end
     : typeclass_instances.
 
   Lemma sim_id {G A} (α : rts G A) :
-    sim eq α α.
+    sim abr_id (fun _ => eq) α α.
   Proof.
-    intros a _ [] a' Ha'. exists a'. split; eauto. reflexivity.
+    intros w a _ [ ] a' Ha'. exists a'. split; eauto. reflexivity.
   Qed.
 
-  Global Instance sim_compose {G A B C RAB RBC RAC} :
-    forall `{!RDecompose RAB RBC RAC} `{!RCompose RAB RBC RAC},
-    @RCompose (rts G A) (rts G B) (rts G C) (sim RAB) (sim RBC) (sim RAC).
+  Global Instance sim_compose {GA GB GC GRAB GRBC A B C RAB RBC RAC} :
+    (forall wab wbc, RDecompose (RAB wab) (RBC wbc) (RAC (wab, wbc))) ->
+    (forall wab wbc, RCompose (RAB wab) (RBC wbc) (RAC (wab, wbc))) ->
+    @RCompose (rts GA A) (rts GB B) (rts GC C)
+      (sim GRAB RAB)
+      (sim GRBC RBC)
+      (sim (abr_compose GRAB GRBC) RAC).
   Proof.
-    intros HRD HRC α β γ Hαβ Hβγ a c Hac.
+    intros HRD HRC α β γ Hαβ Hβγ [wab wbc] a c Hac. red in Hαβ, Hβγ.
     rdecompose Hac as (b & Hab & Hac).
-    rcompose (β b); eauto.
+    rcompose (β b); rauto.
   Qed.
 
   (** ** Externally observable behaviors *)
@@ -293,9 +349,9 @@ Module RTS.
 
   (** Observations are compatible with simulations. *)
 
-  Lemma forever_internal_sim {G A B} (R : rel A B) α β a b :
-    sim (G:=G) R α β ->
-    R a b ->
+  Lemma forever_internal_sim {GA GB A B} (GR : abrel GA GB) (R : klr _ A B) w α β a b :
+    sim GR R α β ->
+    R w a b ->
     forever_internal α a ->
     forever_internal β b \/ obs β b goes_wrong.
   Proof.
@@ -312,13 +368,13 @@ Module RTS.
       econstructor; eauto.
   Qed.
 
-  Lemma reachable_sim {G A B} (R : rel A B) α β a b a' :
-    sim (G:=G) R α β ->
-    R a b ->
+  Lemma reachable_sim {GA GB A B} (GR : abrel GA GB) (R : klr _ A B) w α β a b a' :
+    sim GR R α β ->
+    R w a b ->
     reachable α a a' ->
     exists b',
       reachable β b b' /\
-      (R a' b' \/ β b' goes_wrong).
+      (R w a' b' \/ β b' goes_wrong).
   Proof.
     intros Hαβ Hab Ha'. revert b Hab.
     induction Ha' as [a | a a' a'' Ha' Ha'' IHa'']; eauto.
@@ -329,9 +385,11 @@ Module RTS.
   Qed.
 
   Global Instance behavior_external_sim :
-    Monotonic (@behavior_external) (forallr -, forallr R, behavior_le R ++> impl).
+    Monotonic
+      (@behavior_external)
+      (forallr GR, forallr R, rforall w, behavior_le GR R w ++> impl).
   Proof.
-    intros G A B R a b Hab Ha.
+    intros GA GB GR A B R w a b Hab Ha.
     destruct Ha; inversion Hab; eauto.
   Qed.
 
@@ -339,9 +397,11 @@ Module RTS.
     eapply impl_transport : typeclass_instances.
 
   Global Instance obs_sim :
-    Monotonic (@obs) (forallr -, forallr R, sim R ++> sim R).
+    Monotonic
+      (@obs)
+      (forallr GR, forallr R : klr _, sim GR R ++> sim GR R).
   Proof.
-    intros G A B R α β Hαβ a b Hab ra Hra.
+    intros GA GB GR A B R α β Hαβ w a b Hab ra Hra.
     destruct Hra as [Ha | a' ra Hext Hra Ha' ].
     - edestruct @forever_internal_sim as [Hb | Hb]; eauto.
       + exists diverges. split; eauto. rauto.
@@ -563,14 +623,22 @@ Module RTS.
   Hint Constructors sum.
   Infix "+" := sum : rts_scope.
 
+  (*
   Global Instance sum_sim :
     Monotonic
       (@sum)
-      (forallr -, forallr RA, forallr RB, sim RA ++> sim RB ++> sim (RA + RB)).
+      (forallr GR, forallr RA, forallr RB,
+         sim GR RA ++> sim GR RB ++> sim GR (RA + RB)%klr).
   Proof.
-    intros G A1 A2 RA B1 B2 RB α1 α2 Hα β1 β2 Hβ s1 s2 Hs s1' Hs1'.
-    destruct Hs1'; inversion Hs; transport H; (eexists; split; [eauto | try rauto]).
+    intros GA GB GR A1 A2 RA B1 B2 RB α1 α2 Hα β1 β2 Hβ w s1 s2 Hs s1' Hs1'.
+    destruct Hs1'; inversion Hs.
+    -
+    eapply transport in H.
+    Focus 2. rstep.
+
+ transport H; (eexists; split; [eauto | try rauto]).
   Qed.
+*)
 
   (** *** Commutation with [obs] *)
 
@@ -660,9 +728,9 @@ Module RTS.
   Qed.
 
   Lemma sum_obs {G A B} (α : rts G A) (β : rts G B) :
-    RTS.sim eq (obs (α + β)) (obs α + obs β).
+    RTS.sim abr_id (fun _ => eq) (obs (α + β)) (obs α + obs β).
   Proof.
-    intros s _ [] r Hr.
+    intros w s _ [ ] r Hr.
     exists r; split; [ | rauto].
     destruct Hr as [Hs | s' r Hrext Hr Hs'].
     - apply sum_forever_internal_inv in Hs as [(a & ? & H) | (b & ? & H)]; subst.
@@ -677,9 +745,9 @@ Module RTS.
   Qed.
 
   Lemma obs_sum {G A B} (α : rts G A) (β : rts G B) :
-    RTS.sim eq (obs α + obs β) (obs (α + β)).
+    RTS.sim abr_id (fun _ => eq) (obs α + obs β) (obs (α + β)).
   Proof.
-    intros s _ [] r Hr.
+    intros w s _ [ ] r Hr.
     exists r; split; [ | rauto].
     destruct Hr as [a ra Hra | b rb Hrb].
     - destruct Hra.
